

(1) form a partial differential equation by eliminating  $a, b, c$  from  $\frac{x^2}{a^2} + \frac{y^2}{b^2} + \frac{z^2}{c^2} = 1$ .

Given,  $\frac{x^2}{a^2} + \frac{y^2}{b^2} + \frac{z^2}{c^2} = 1$  — (i)

Here, the number of arbitrary constant is more than the number of independent variable.

Now, Differentiating eq<sup>n</sup> (i) partially w.r.t  $x$  we get,

$$\frac{2x}{a^2} + \frac{2z}{c^2} \cdot \frac{dz}{dx} = 0$$

$$\Rightarrow \frac{x}{a^2} + \frac{z}{c^2} \cdot \frac{dz}{dx} = 0 \text{ — (2)}$$

Differentiating eq<sup>n</sup> (i) partially w.r.t  $y$  we get,

$$\frac{2y}{b^2} + \frac{2z}{c^2} \cdot \frac{dz}{dy} = 0$$

$$\Rightarrow \frac{y}{b^2} + \frac{z}{c^2} \cdot \frac{dz}{dy} = 0 \text{ — (3)}$$

Differentiating eq<sup>n</sup> (2) partially w.r.t  $x$  we get,

$$\frac{1}{a^2} + \frac{1}{c^2} \left[ P \cdot \frac{dz}{dx} + Z \cdot \frac{dP}{dx} \right] = 0$$

$$\Rightarrow \frac{1}{a^2} + \frac{P^2}{c^2} + \frac{ZP}{c^2} = 0 \text{ — (4)}$$

Differentiating eq<sup>n</sup> (3) partially w.r.t  $y$  we get,

$$\frac{1}{b^2} + \frac{1}{c^2} \left[ Q \cdot \frac{dz}{dy} + Z \cdot \frac{dQ}{dy} \right] = 0$$

$$\Rightarrow \frac{1}{b^2} + \frac{Q^2}{c^2} + \frac{ZQ}{c^2} = 0 \text{ — (5)}$$

Differentiating eq<sup>n</sup> (5) partially w.r.t  $y$  we get,

$$\frac{1}{c^2} \left[ P \cdot \frac{dz}{dy} + Z \cdot \frac{dP}{dy} \right] = 0$$

$$\Rightarrow \frac{PQ}{c^2} + \frac{ZS}{c^2} = 0 \text{ — (6)}$$

From eq<sup>n</sup> (6) we can get,

$$PQ + ZS = 0 \text{ (Ans)}$$

(2) form a partial differential equation by eliminating the arbitrary functions  $f$  and  $g$  from  $Z = y \cdot f(x) + x \cdot g(y)$

Given,  $Z = y \cdot f(x) + x \cdot g(y)$  — (i)

Now, Differentiating eq<sup>n</sup> (i) partially w.r.t  $x$  we get,

$$\frac{\partial Z}{\partial x} = y f'(x) + g(y) \Rightarrow P = y f'(x) + g(y) \text{ — (2)}$$

Differentiating eq<sup>n</sup> (1) partially w.r.t y we get,

$$\frac{\partial z}{\partial y} = f(x) + xg'(y) \Rightarrow z = f(x) + xg(y) \quad \text{--- (3)}$$

Multiply x and y in both sides of eq<sup>n</sup> (2) and eq<sup>n</sup> (3) respectively we can get,

$$xp = xyf'(x) + xg(y) \quad \text{--- (4)}$$

$$xy = yf(x) + xyg'(y) \quad \text{--- (5)}$$

Now, adding eq<sup>n</sup> (4) and (5) we can get,

$$xp + yq = xy[f'(x) + g'(y)] + xg(y) + yf(x)$$

$$\Rightarrow xp + yq = xy[f'(x) + g'(y)] + z \quad \text{--- (6)}$$

Differentiating eq<sup>n</sup> (2) partially w.r.t y we can get,

$$\frac{\partial p}{\partial y} = f'(x) + g'(y)$$

$$\Rightarrow s = f'(x) + g'(y)$$

Now, substituting this value in eq<sup>n</sup> (6) we can get,

$$xp + yq = xys + z \quad (\text{Ans})$$

③ If  $f(x+ay) + \phi(x-ay)$ , prove that  $\frac{\partial^2 z}{\partial y^2} = a^2 \left( \frac{\partial^2 z}{\partial x^2} \right)$

Given,  $z = f(x+ay) + \phi(x-ay)$

$$\frac{\partial z}{\partial x} = f'(x+ay) + \phi'(x-ay)$$

$$\frac{\partial^2 z}{\partial x^2} = f''(x+ay) + \phi''(x-ay)$$

$$\text{Now } \frac{\partial z}{\partial y} = af'(x+ay) - a\phi'(x-ay)$$

$$\frac{\partial^2 z}{\partial y^2} = a^2 f''(x+ay) + a^2 \phi''(x-ay)$$

$$\frac{\partial^2 z}{\partial y^2} = a^2 [f''(x+ay) + \phi''(x-ay)]$$

$$\Rightarrow \frac{\partial^2 z}{\partial y^2} = a^2 \left( \frac{\partial^2 z}{\partial x^2} \right) \quad (\text{proved})$$

$$\Rightarrow \frac{\partial^2 z}{\partial y^2} = a^2 \left( \frac{\partial^2 z}{\partial x^2} \right) \quad (\text{proved})$$

④ form a partial differential equation by eliminating the arbitrary functions from  $f\left(\frac{x-a}{z-c}, \frac{y-b}{z-c}\right) = 0$ .

$$(\text{Given } f\left(\frac{x-a}{z-c}, \frac{y-b}{z-c}\right) = 0)$$

$$u = \frac{x-a}{z-c}, \quad v = \frac{y-b}{z-c}$$

$$p = \frac{\partial \left( \frac{x-a}{z-c} \right)}{\partial x} \cdot \frac{\partial \left( \frac{y-b}{z-c} \right)}{\partial y}$$

$$\Rightarrow p = - \left[ \frac{(z-c) \cdot 0 - (x-a)}{(z-c)^2} \cdot \frac{(z-c) - (y-b) \cdot 0}{(z-c)^2} \right]$$

$$\Rightarrow p = \frac{(x-a)(z-c)}{(z-c)^4}$$

$$\Rightarrow p = \frac{x-a}{(z-c)^3}$$

$$q = - \frac{\partial \left( \frac{x-a}{z-c} \right)}{\partial x} \cdot \frac{\partial \left( \frac{y-b}{z-c} \right)}{\partial z}$$

$$\Rightarrow q = - \left[ \frac{(z-c) - (x-a) \cdot 0}{(z-c)^2} \cdot \frac{(z-c) \cdot 0 - (y-b)}{(z-c)^2} \right]$$

$$\Rightarrow q = \frac{(z-c)(y-b)}{(z-c)^4}$$

$$\Rightarrow q = \frac{y-b}{(z-c)^3}$$

$$R = \frac{\partial \left( \frac{x-a}{z-c} \right)}{\partial x} \cdot \frac{\partial \left( \frac{y-b}{z-c} \right)}{\partial y}$$

$$\Rightarrow R = \frac{(z-c) - (x-a) \cdot 0}{(z-c)^2} \cdot \frac{(z-c) - (y-b) \cdot 0}{(z-c)^2}$$

$$\Rightarrow R = \frac{(z-c)^2}{(z-c)^4}$$

$$\Rightarrow R = \frac{1}{(z-c)^2}$$

Therefore, the required PDE is

$$\frac{(x-a)}{(z-c)^3} p + \frac{(y-b)}{(z-c)^3} q = \frac{1}{(z-c)^2}$$

$$\Rightarrow \boxed{(x-a)p + (y-b)q = (z-c) \text{ (Ans)}}.$$

⑤ Solve the PDE  $y^2p - xyq = x(z - 2y)$ .

Given,  $y^2p - xyq = x(z - 2y)$  ——— ①

Here,  $P = y^2$ ,  $Q = -xy$ ,  $R = x(z - 2y)$

Now, the Lagrange's auxiliary eqn is  $\frac{dx}{y^2} = \frac{dy}{-xy} = \frac{dz}{x(z - 2y)}$  ——— ②

By taking the first and second ratio from eqn ② we get,

$$\frac{dx}{y^2} = \frac{dy}{-xy} \Rightarrow -\int x dx = \int y dy$$

$$\Rightarrow -\frac{x^2}{2} + c_1 = \frac{y^2}{2} + c_2 \Rightarrow [x^2 + y^2 = c] \text{ ——— ③}$$

By taking the second and last ratio from eqn ② we get

$$\frac{dy}{-xy} = \frac{dz}{x(z - 2y)}$$

$$\Rightarrow \frac{dy}{y} = \frac{dz}{2y - z} \Rightarrow \frac{dz}{dy} = \frac{2y - z}{y} \Rightarrow \frac{dz}{dy} = 2 - \frac{z}{y}$$

$$\Rightarrow \frac{dz}{dy} + \frac{z}{y} = 2$$

Integrating factor

$$= e^{\int \frac{1}{y} dy} = e^{\ln y} = y$$

$$\text{Now, } yz = \int 2 \cdot y \cdot dy$$

$$\Rightarrow yz = 2 \cdot \frac{y^2}{2} + K$$

$$\Rightarrow yz - y^2 = K \text{ ——— ④}$$

Therefore, the required solution is  $\phi(x^2 + y^2, yz - y^2) = 0$  (Ans)

⑥ Solve the PDE  $py + qx = xyz^2(x^2 - y^2)$ .

Given,  $py + qx = xyz^2(x^2 - y^2)$  ——— ①

Here,  $P = y$ ,  $Q = x$ ,  $R = xyz^2(x^2 - y^2)$

Now, the Lagrange's auxiliary eqn is

$$\frac{dx}{y} = \frac{dy}{x} = \frac{dz}{xyz^2(x^2 - y^2)} \text{ ——— ②}$$

By taking first and second ratio from eqn ② we get,

$$\frac{dx}{y} = \frac{dy}{x} \Rightarrow \int x dx = \int y dy$$

$$\Rightarrow \frac{x^2}{2} + c_1 = \frac{y^2}{2} + c_2$$

$$\Rightarrow x^2 - y^2 = c \text{ ——— ③}$$

By taking second and last ratio from eqn ② we get,

$$\frac{dy}{x} = \frac{dz}{xyz^2(x^2 - y^2)}$$

$$\Rightarrow dy = \frac{dz}{yz^2(x^2 - y^2)}$$



$$\Rightarrow \int y \, dy = \int \frac{dz}{z} \cdot c$$

$$\Rightarrow \frac{y^2}{2} + c_3 = -\frac{1}{2}c + c_4$$

$$\Rightarrow \frac{y^2}{2} + \frac{1}{z(x^2 - y^2)} = k \quad \text{--- (4)}$$

Therefore, the required solution is  $\phi(x^2 - y^2, \frac{y^2}{2} + \frac{1}{z(x^2 - y^2)}) = 0$ .  
(Ans).

7) Solve the PDE  $(y-z)p + (z-x)q = (x-y)$ .

Given,  $(y-z)p + (z-x)q = (x-y)$  --- (1)

Here,  $P = y-z$ ,  $Q = z-x$ ,  $R = x-y$ .

Now, the Lagrange's auxiliary eq<sup>n</sup> is

$$\frac{dx}{y-z} = \frac{dy}{z-x} = \frac{dz}{x-y} \quad \text{--- (2)}$$

Choosing 1, 1, 1 as multipliers of each fraction for eq<sup>n</sup> (2) we get,

$$\frac{dx}{y-z} = \frac{dy}{z-x} = \frac{dz}{x-y} = \frac{dx + dy + dz}{y-z + z-x + x-y}$$

$$\Rightarrow dx + dy + dz = 0$$

$$\Rightarrow \int dx + \int dy + \int dz = 0$$

$$\Rightarrow x + y + z + c_1 + c_2 + c_3 = 0$$

$$\Rightarrow x + y + z = c \quad \text{--- (3)}$$

Choosing  $x, y, z$  as multipliers of each fraction for eq<sup>n</sup> (2) we get,

$$\frac{x \, dx}{x(y-z)} = \frac{y \, dy}{y(z-x)} = \frac{z \, dz}{z(x-y)} = \frac{x \, dx + y \, dy + z \, dz}{xy - xz + yz - xy + xz - yz}$$

$$\Rightarrow x \, dx + y \, dy + z \, dz = 0$$

$$\Rightarrow \int x \, dx + \int y \, dy + \int z \, dz = 0$$

$$\Rightarrow \frac{x^2}{2} + \frac{y^2}{2} + \frac{z^2}{2} + c_4 + c_5 + c_6 = 0$$

$$\Rightarrow x^2 + y^2 + z^2 = k \quad \text{--- (4)}$$

Therefore, the required solution is

$$\phi(x + y + z, x^2 + y^2 + z^2) = 0 \quad \text{(Ans)}$$

8) Solve the PDE  $(y+z)p + (z+x)q = (x+y)$

Given  $(y+z)p + (z+x)q = (x+y)$  --- (1)

Here,  $P = y+z$ ,  $Q = z+x$ ,  $R = x+y$

Now, the Lagrange's auxiliary eq<sup>n</sup> is  $\frac{dx}{y+z} = \frac{dy}{z+x} = \frac{dz}{x+y}$  --- (2)

choosing 1, -1, 0 as multipliers of each fraction of eq<sup>n</sup> (1) we get,

$$\frac{dx}{y+z} = \frac{-dy}{-(z+x)} = \frac{0}{0} = \frac{dx-dy}{y+z-z-x} = \frac{dx-dy}{x-y}$$

choosing 0, 1, -1 as multipliers of each fraction of eq<sup>n</sup> (2) we get,

$$\frac{0}{0} = \frac{dy}{z+x} = \frac{-dz}{-(x+y)} = \frac{dy-dz}{z+x-x-y} = \frac{dy-dz}{z-y} \quad \text{--- (4)}$$

choosing 1, 1, 1 as multipliers of each fraction of eq<sup>n</sup> (2) we get,

$$\frac{dx}{y+z} = \frac{dy}{z+x} = \frac{dz}{x+y} = \frac{dx+dy+dz}{2x+2y+2z} \quad \text{--- (5)}$$

$$\text{Now } \frac{dx-dy}{x-y} = \frac{dy-dz}{z-y} = \frac{dx+dy+dz}{2x+2y+2z} \quad \text{--- (6)}$$

By taking the first and second ratio from eq<sup>n</sup> (6) we get,

$$\begin{aligned} \frac{dx-dy}{x-y} &= \frac{dy-dz}{z-y} \\ \Rightarrow \frac{dx-dy}{x-y} &= \frac{dy-dz}{y-z} \Rightarrow \int \frac{d(x-y)}{x-y} = \int \frac{d(y-z)}{y-z} \\ &\Rightarrow \ln|x-y| + \ln c_1 = \ln|y-z| + \ln c_2 \\ &\Rightarrow \ln \left| \frac{x-y}{y-z} \right| = \ln \left| \frac{c_2}{c_1} \right| \\ &\Rightarrow \frac{x-y}{y-z} = c \quad \text{--- (7)} \end{aligned}$$

By taking the first and third ratio from eq<sup>n</sup> (6) we get,

$$\begin{aligned} \frac{dx-dy}{x-y} &= \frac{dx+dy+dz}{2x+2y+2z} \\ \Rightarrow \frac{dx-dy}{-(x-y)} &= \frac{dx+dy+dz}{2(x+y+z)} \\ \Rightarrow -\int \frac{d(x-y)}{(x-y)} &= \int \frac{d(x+y+z)}{2(x+y+z)} \\ \Rightarrow -\ln|x-y| + \ln c_3 &= \frac{1}{2} \ln|x+y+z| + \ln c_4 \\ \Rightarrow \frac{1}{2} \ln|x+y+z| + \ln|x-y| &= \ln c_3 - \ln c_4 \\ \Rightarrow \ln|(x+y+z)^{1/2}(x-y)| &= \ln \left| \frac{c_3}{c_4} \right| \\ \Rightarrow \sqrt{x+y+z}(x-y) &= k \quad \text{--- (8)} \end{aligned}$$

Therefore, the required solution is

$$\phi\left(\frac{x-y}{y-z}, \sqrt{x+y+z}(x-y)\right) = 0 \quad (\text{Ans}).$$

Q1) Solve the partial differential equation  
 $px(x+y) - qy(x+y) + (x-y)(2x+2y+z) = 0$

Given,  $px(x+y) - qy(x+y) + (x-y)(2x+2y+z) = 0$

$$\rightarrow px(x+y) - qy(x+y) = -(x-y)(2x+2y+z) \quad \text{--- (1)}$$

Here,  $p = x(x+y)$ ,  $Q = -y(x+y)$ ,  $R = -(x-y)(2x+2y+z)$

Now, the Lagrange's auxiliary eqn is

$$\frac{dx}{x(x+y)} = \frac{dy}{-y(x+y)} = \frac{dz}{-(x-y)(2x+2y+z)} \quad \text{--- (2)}$$

By taking first and second ratio from eqn (2) we get,

$$\begin{aligned} \frac{dx}{x(x+y)} &= \frac{dy}{-y(x+y)} \\ \Rightarrow \frac{dx}{x} &= \frac{dy}{-y} \Rightarrow \int \frac{dx}{x} = -\int \frac{dy}{y} \\ &\Rightarrow \ln x + \ln c_1 = -\ln y + \ln c_2 \\ &\Rightarrow \ln x + \ln y = \ln c_2 - \ln c_1 \\ &\Rightarrow \ln |xy| = \ln \left| \frac{c_2}{c_1} \right| \\ &\Rightarrow xy = c \quad \text{--- (3)} \end{aligned}$$

Choosing 1, 1, 0 as multipliers of each fraction of eqn (2) we get,

$$\frac{dx}{x(x+y)} = \frac{dy}{-y(x+y)} = \frac{0}{0} = \frac{dx+dy}{x(x+y)-y(x+y)} \quad \text{--- (4)}$$

Choosing 1, 1, 1 as multipliers of each fraction of eqn (2) we get,

$$\frac{dx}{x(x+y)} = \frac{dy}{-y(x+y)} = \frac{dz}{-(x-y)(2x+2y+z)} = \frac{dx+dy+dz}{x(x+y)-y(x+y)-(x-y)(2x+2y+z)} \quad \text{--- (5)}$$

$$\text{Now, } \frac{dx+dy}{x(x+y)-y(x+y)} = \frac{dx+dy+dz}{x(x+y)-y(x+y)-(x-y)(2x+2y+z)}$$

$$\Rightarrow \frac{dx+dy}{(x+y)(x-y)} = \frac{dx+dy+dz}{(x+y)(x-y)-(x-y)(2x+2y+z)}$$

$$\Rightarrow \frac{dx+dy}{(x+y)(x-y)} = \frac{dx+dy+dz}{(x-y)(x+y-2x-2y-z)}$$

$$\Rightarrow \frac{dx+dy}{x+y} = \frac{dx+dy+dz}{-(x+y+z)}$$

$$\Rightarrow \int \frac{d(x+y)}{x+y} = - \int \frac{d(x+y+z)}{x+y+z}$$

$$\Rightarrow \ln|x+y| + \ln c_3 = -\ln|x+y+z| + \ln c_4$$

$$\Rightarrow \ln|x+y| + \ln|x+y+z| = \ln c_4 - \ln c_3$$

$$\Rightarrow \ln|(x+y)(x+y+z)| = \ln \left( \frac{c_4}{c_3} \right)$$

$$\Rightarrow (x+y)(x+y+z) = k \quad \text{--- (6)}$$

Therefore, the required solution is

$$\phi(xy, (x+y)(x+y+z)) = 0$$

(11) Find the complete integral of  $16p^2z^2 + 9q^2z^2 + 4z^2 - 4 = 0$

$$\text{Given, } 16p^2z^2 + 9q^2z^2 + 4z^2 - 4 = 0 \quad \text{--- (1)}$$

$$\text{Here, } f(x, y, z, p, q) = 16p^2z^2 + 9q^2z^2 + 4z^2 - 4 = 0$$

$$\text{Now } f_x = 0, \quad f_y = 0, \quad f_z = 32p^2z + 18q^2z + 8z,$$

$$f_p = 32pz^2, \quad f_q = 18qz^2$$

Now, Charpit's auxiliary eq<sup>n</sup> is

$$\frac{dp}{32p^3z + 18pq^2z + 8pz} = \frac{dq}{32p^2qz + 18q^3z + 8qz} = \frac{dz}{-32p^2z^2 - 18q^2z^2} = \frac{dx}{-32pz^2}$$

By taking first and second ratio of eq<sup>n</sup> (2)

$$\text{we get, } \frac{dp}{32p^3z + 18pq^2z + 8pz} = \frac{dq}{32p^2qz + 18q^3z + 8qz}$$

$$\Rightarrow \frac{dp}{p(32p^2z + 18q^2z + 8z)} = \frac{dq}{q(32p^2z + 18q^2z + 8z)}$$

$$\Rightarrow \int \frac{dp}{p} = \int \frac{dq}{q}$$

$$\Rightarrow \ln p + \ln c_1 = \ln q + \ln c_2$$

$$\Rightarrow \ln p - \ln q = \ln c_2 - \ln c_1$$

$$\Rightarrow \ln\left(\frac{p}{q}\right) = \ln\left(\frac{c_2}{c_1}\right) \Rightarrow \frac{p}{q} = a \Rightarrow p = aq$$

Now, putting this value in eq<sup>n</sup> (1) we get,

$$16a^2q^2z^2 + 9q^2z^2 + 4z^2 - 4 = 0$$

$$\Rightarrow q^2z^2(16a^2 + 9) = 4 - 4z^2$$

$$\Rightarrow q^2z^2 = \frac{4 - 4z^2}{16a^2 + 9}$$



$$\Rightarrow q^2 = \frac{4}{z^2} \left[ \frac{1-z^2}{16a^2+9} \right]$$

$$\Rightarrow q = \frac{2}{z} \sqrt{\frac{1-z^2}{16a^2+9}}$$

$$\Rightarrow q = \frac{2}{\sqrt{16a^2+9}} \cdot \frac{\sqrt{1-z^2}}{z}$$

$$\text{Now } p = \frac{2a}{\sqrt{16a^2+9}} \cdot \frac{\sqrt{1-z^2}}{z}$$

$$\text{Now, } dz = p dx + q dy$$

$$\Rightarrow dz = \left( \frac{2a}{\sqrt{16a^2+9}} \cdot \frac{\sqrt{1-z^2}}{z} \right) dx + \left( \frac{2}{\sqrt{16a^2+9}} \cdot \frac{\sqrt{1-z^2}}{z} \right) dy$$

$$\Rightarrow \frac{z}{\sqrt{1-z^2}} dz = \frac{2}{\sqrt{16a^2+9}} (a dx + dy)$$

$$\Rightarrow \int \frac{z \cdot dz}{\sqrt{1-z^2}} = \frac{2}{\sqrt{16a^2+9}} [a \int dx + \int dy]$$

$$\Rightarrow - \int \frac{v dv}{v} = \frac{2}{\sqrt{16a^2+9}} (ax + y) + b$$

$$\Rightarrow -\sqrt{1-z^2} = \frac{2}{\sqrt{16a^2+9}} (ax + y) + b$$

$$\Rightarrow \frac{2}{\sqrt{16a^2+9}} (ax + y) + \sqrt{1-z^2} = b \quad (\text{Ans})$$

(ii) find the complete integral of  $p^2 + q^2 - 2px - 2qy + 2xy = 0$

$$\text{Given } p^2 + q^2 - 2px - 2qy + 2xy = 0 \quad \text{--- (1)}$$

$$\text{Here } f(x, y, z, p, q) = p^2 + q^2 - 2px - 2qy + 2xy = 0$$

$$\text{Now, } f_x = -2p + 2y, \quad f_y = -2q + 2x, \quad f_z = 0$$

$$f_p = 2p - 2x, \quad f_q = 2q - 2y$$

Now, Charpit's auxiliary eqn is

$$\frac{dp}{-2p+2y} = \frac{dq}{-2q+2x} = \frac{dz}{-2p^2+2p^2-2q^2+2q^2} = \frac{dx}{-2p+2x} = \frac{dy}{-2q+2y} = 0 \quad \text{--- (2)}$$

By taking first and second ratio from eqn (2)

$$\frac{dp}{-2p+2y} = \frac{dq}{-2q+2x} = \frac{dp+dx}{2(-p+y-q+x)} \quad \text{--- (3)}$$

By taking fourth and fifth ratio from eq<sup>n</sup> ② we get,

$$\frac{dx}{-2p+2x} = \frac{dy}{-2q+2y} = \frac{dx+dy}{2(-p+x-q+y)} \quad \text{--- (4)}$$

From eq<sup>n</sup> ③ and ④ we get

$$\frac{dp+dq}{2(-p+q-x+y)} = \frac{dx+dy}{2(-p+x-q+y)}$$

$$\Rightarrow \int d(p+q) = \int d(x+y)$$

$$\Rightarrow p+q = x+y+a$$

$$\Rightarrow p-x+q-y = a \quad \text{--- (5)}$$

From eq<sup>n</sup> ① we can write

$$(p-x)^2 + (q-y)^2 = (x-y)^2 \quad \text{--- (6)}$$

From eq<sup>n</sup> ⑤,  $q-y = a - (p-x)$

Putting this value in eq<sup>n</sup> ⑥ we can get,

$$(p-x)^2 + [a - (p-x)]^2 = (x-y)^2$$

$$\Rightarrow (p-x)^2 + a^2 + (p-x)^2 - 2a(p-x) = (x-y)^2$$

$$\Rightarrow 2(p-x)^2 - 2a(p-x) + \{a^2 - (x-y)^2\} = 0$$

$$\Rightarrow p-x = \frac{2a \pm \sqrt{4a^2 - 8\{a^2 - (x-y)^2\}}}{4}$$

$$\Rightarrow p = x + \frac{1}{2} [a \pm \sqrt{2(x-y)^2 - a^2}]$$

From eq<sup>n</sup> ⑤ we get,  $q = a + y - p + x$

$$\Rightarrow q = a + y - (p-x)$$

$$\Rightarrow q = y + a - \frac{2a \pm \sqrt{4a^2 - 8\{a^2 - (x-y)^2\}}}{4}$$

$$\Rightarrow q = y + \frac{2a \pm \sqrt{4a^2 - 8\{a^2 - (x-y)^2\}}}{4}$$

$$\Rightarrow q = y + \frac{1}{2} [a \pm \sqrt{2(x-y)^2 - a^2}]$$

Putting these values of  $p$  and  $q$  in  $dz = p dx + q dy$  we get,

$$dz = x dx + y dy + \frac{1}{2} [a \pm \sqrt{2(x-y)^2 - a^2}] dx + \frac{1}{2} [a \pm \sqrt{2(x-y)^2 - a^2}] dy$$

$$\Rightarrow dz = x dx + y dy + \frac{a}{2} (dx + dy) \pm \frac{1}{2} \sqrt{2(x-y)^2 - a^2} (dx - dy)$$

$$\Rightarrow \int dz = \int x dx + \int y dy + \frac{a}{2} \int d(x+y) + \frac{1}{\sqrt{2}} \int \sqrt{(x-y)^2 - \frac{a^2}{2}} (dx - dy)$$

$$\Rightarrow Z = \frac{x^2}{2} + \frac{y^2}{2} + \frac{a}{2}(x+y) + \frac{1}{\sqrt{2}} \left( \frac{x-y}{2} \sqrt{(x-y)^2 - \frac{a^2}{2}} - \frac{a^2}{4} \log \left[ (x-y) + \sqrt{(x-y)^2 - \frac{a^2}{2}} \right] \right)$$

$$\Rightarrow Z = \frac{x^2+y^2}{2} + \frac{a(x+y)}{2} + \frac{1}{\sqrt{2}} \left( \frac{x-y}{2} \sqrt{(x-y)^2 - \frac{a^2}{2}} - \frac{a^2}{4} \log \left[ (x-y) + \sqrt{(x-y)^2 - \frac{a^2}{2}} \right] \right)$$

(12) Solve the PDE  $p^2 q^2 + x^2 y^2 = x^2 q^2 (x^2 + y^2)$  (Ans)

Given ~~PDE~~  $p^2 q^2 + x^2 y^2 = x^2 q^2 (x^2 + y^2)$

$$\Rightarrow p^2 q^2 + x^2 y^2 = x^4 q^2 + x^2 y^2 q^2$$

$$\Rightarrow p^2 q^2 = x^4 q^2 + x^2 y^2 (q^2 - 1) \quad \text{--- (1)}$$

Dividing  $q^2$  both sides of the eq<sup>n</sup> (1) we get,

$$p^2 = x^4 + x^2 y^2 \left( 1 - \frac{1}{q^2} \right)$$

$$\Rightarrow p^2 - x^4 = x^2 y^2 \left( 1 - \frac{1}{q^2} \right) \quad \text{--- (2)}$$

Dividing  $x^2$  both sides of the eq<sup>n</sup> (2) we get,

$$\frac{p^2}{x^2} - x^2 = y^2 \left( 1 - \frac{1}{q^2} \right)$$

$$\Rightarrow \frac{p^2}{x^2} - x^2 = y^2 - \frac{y^2}{q^2} = a^2$$

Now,  $\frac{p^2}{x^2} - x^2 = a^2$

$$\Rightarrow \frac{p^2}{x^2} = a^2 + x^2$$

$$\Rightarrow p^2 = (a^2 + x^2) x^2$$

$$\Rightarrow p = x \sqrt{a^2 + x^2}$$

$$y^2 - \frac{y^2}{q^2} = a^2$$

$$\Rightarrow \frac{y^2}{q^2} = y^2 - a^2$$

$$\Rightarrow q^2 = \frac{y^2}{y^2 - a^2}$$

$$\Rightarrow q = \frac{y}{\sqrt{y^2 - a^2}}$$

Now,  $dz = p dx + q dy$

$$\Rightarrow dz = x \sqrt{a^2 + x^2} dx + \frac{y}{\sqrt{y^2 - a^2}} dy$$

$$\Rightarrow \int dz = \int \sqrt{a^2 + x^2} x dx + \int \frac{y dy}{\sqrt{y^2 - a^2}}$$

$$\Rightarrow \int dz = \int u \cdot v du + \int \frac{v dv}{v} \quad \text{uf } v^2 = a^2 + x^2$$

$$\Rightarrow \int dz = \int u^2 du + \int dv \quad \Rightarrow 2v dv = 2x dx$$

$$\Rightarrow Z = \frac{v^3}{3} + v + b \quad \Rightarrow v dv = x dx$$

$$\Rightarrow Z = \frac{1}{3} (a^2 + x^2)^{3/2} + \sqrt{y^2 - a^2} + b \quad (\text{Ans})$$

- (13) Find the complementary function of  $(D_x + 2D_y - 3)Z = 0$   
 $(D_x + D_y - 1)Z = 0$ .

Given  $(D_x + 2D_y - 3)(D_x + D_y - 1)Z = 0$

Here  $a = 1, b = 2, c = -3, \quad a = 1, b = 1, c = -1$

So  $Z = e^{3x} \phi(y + 2x) + e^x \phi(y - x) \quad (\text{Ans})$

- (14) Find the complementary function of  
 $(D_x^3 - D_x^2 D_y - 8D_x D_y^2 + 12D_y^3)Z = 0$ .

Given,  $(D_x^3 - D_x^2 D_y - 8D_x D_y^2 + 12D_y^3)Z = 0$

Take  $D_x = m, D_y = 1$

So auxiliary eq<sup>n</sup> is  $m^3 - m^2 - 8m + 12 = 0$

$\Rightarrow m = -3, 2, 2$

$m_1 = -3, m_2 = 2, m_3 = 2$

So,  $Z = \phi_1(y - 3x) + \phi_2(y + 2x) + x \phi_3(y + 2x) \quad (\text{Ans})$

- (15) Find the complementary function of  
 $(D_x^4 - D_y^4)Z = 0$

Given  $(D_x^4 - D_y^4)Z = 0$

Take  $D_x = m, D_y = -1$

So auxiliary eq<sup>n</sup> is  $(m^4 - 1) = 0$

$\Rightarrow m = 1, -1, i, -i$

So  $Z = \phi_1(y + x) + \phi_2(y - x) + \phi_3(y + ix) + \phi_4(y - ix) + i[\phi_4(y + ix) - \phi_4(y - ix)] \quad (\text{Ans})$



\* Find the complete integral of  $p^2 + q^2 - 2px - 2qy + 2xy = 0$

Soln:- Given equation is,

$$f(x, y, z, p, q) = p^2 + q^2 - 2px - 2qy + 2xy = 0 \quad \text{--- (1)}$$

Charpit's auxiliary equations are,

$$\frac{dp}{\frac{\partial f}{\partial x} + p \frac{\partial f}{\partial z}} = \frac{dq}{\frac{\partial f}{\partial y} + q \frac{\partial f}{\partial z}} = \frac{dz}{-p \frac{\partial f}{\partial p} - q \frac{\partial f}{\partial q}} = \frac{dx}{-\frac{\partial f}{\partial p}} = \frac{dy}{-\frac{\partial f}{\partial q}}$$

$$\frac{dp}{-2p + 2y} = \frac{dq}{-2q + 2x} = \frac{dz}{-2p^2 + 2xp - 2q^2 + 2qy} = \frac{dx}{2x - 2p} = \frac{dy}{2y - 2q}$$

$$\Rightarrow \frac{dp + dq}{-2p + 2y - 2q + 2x} = \frac{dx + dy}{2x - 2p + 2y - 2q}$$

$$\Rightarrow dp + dq = dx + dy$$

Integrating the above equation,

$$\Rightarrow p + q = x + y + \text{Constant}$$

$$\Rightarrow (p - x) + (q - y) = a \quad \text{--- (2)}$$

Re-writing equation - (1) we get,

$$p^2 + q^2 - 2px - 2qy + x^2 + y^2 = x^2 + y^2 - 2xy$$

$$\Rightarrow (p - x)^2 + (q - y)^2 = (x - y)^2 \quad \text{--- (3)}$$

from eqn (2) and (3)

$$q - y = a - (p - x)$$

$$\Rightarrow (p - x)^2 + [a - (p - x)]^2 = (x - y)^2$$

$$\Rightarrow (p - x)^2 + a^2 + (p - x)^2 - 2a(p - x) = (x - y)^2$$

$$\Rightarrow 2(p - x)^2 - 2a(p - x) + \{a^2 - (x - y)^2\} = 0$$

$$\Rightarrow p - x = \frac{2a \pm \sqrt{4a^2 - 4 \cdot 2 \{a^2 - (x - y)^2\}}}{4}$$

$$\Rightarrow P = x + \frac{1}{2}[a \pm \sqrt{2(x-y)^2 - a^2}]$$

$$\Rightarrow Q = a + y - P + x$$

$$= a + y + x - x - \frac{1}{2}[a \pm \sqrt{2(x-y)^2 - a^2}]$$

$$= y + \frac{1}{2}[a \mp \sqrt{2(x-y)^2 - a^2}]$$

putting the values of P and Q in

$dz = Pdx + Qdy$ , we get,

$$\Rightarrow dz = x dx + y dy + \frac{1}{2}[a \pm \sqrt{2(x-y)^2 - a^2}](dx - dy)$$

Integration,

$$\Rightarrow z = \frac{x^2}{2} + \frac{y^2}{2} + \int \frac{1}{2}[a \pm \sqrt{2z^2 - a^2}] dz$$

$$= \frac{x^2}{2} + \frac{y^2}{2} + \int \frac{1}{2}[a \pm \sqrt{z^2 - (\frac{a}{\sqrt{2}})^2}] dz$$

$$= \frac{x^2}{2} + \frac{y^2}{2} + \frac{1}{2} \left[ a \pm \sqrt{2} \cdot \sqrt{z^2 - (\frac{a}{\sqrt{2}})^2} \right]$$

$$= \frac{x^2}{2} + \frac{y^2}{2} + \frac{1}{2} \left[ a z \pm \sqrt{2} \left\{ \frac{z}{2} \sqrt{z^2 - (\frac{a}{\sqrt{2}})^2} - \frac{a^2}{2^2} \ln \left| z + \sqrt{z^2 - (\frac{a}{\sqrt{2}})^2} \right| \right\} \right]$$

$$= \frac{x^2}{2} + \frac{y^2}{2} + \frac{1}{2} a(x-y) \pm \frac{1}{\sqrt{2}} \left\{ \frac{x-y}{2} \sqrt{(x-y)^2 - \frac{a^2}{2}} - \frac{a^2}{4} \ln \left| (x-y) + \sqrt{(x-y)^2 - \frac{a^2}{2}} \right| \right\}$$

(Ans.)

$$(08) x^2(y-z)p + y^2(z-x)q = z^2(x-y)$$

Soln.

$$\text{Hence } P = x^2(y-z)$$

$$Q = y^2(z-x)$$

$$R = z^2(x-y)$$

Hence, the Lagrange's auxiliary equation is,

$$\frac{dx}{x^2(y-z)} = \frac{dy}{y^2(z-x)} = \frac{dz}{z^2(x-y)} \quad \text{--- (1)}$$

Choosing  $\frac{1}{x}, \frac{1}{y}, \frac{1}{z}$  as multipliers of each fraction of equation (1), we get

$$\frac{\frac{1}{x} dx}{x(y-z)} = \frac{\frac{1}{y} dy}{y^2(z-x)} = \frac{\frac{1}{z} dz}{z^2(x-y)} = \frac{\frac{dx}{x} + \frac{dy}{y} + \frac{dz}{z}}{\cancel{x(y-z)} + \cancel{xz} + \cancel{yz} + \cancel{xy} + \cancel{xz} + \cancel{xy}}$$

$$\Rightarrow \frac{dx}{x} + \frac{dy}{y} + \frac{dz}{z} = 0$$

Integration,

$$\Rightarrow \int \frac{dx}{x} + \int \frac{dy}{y} + \int \frac{dz}{z} = 0$$

$$\Rightarrow \ln x + \ln y + \ln z = \ln C$$

$$\Rightarrow \boxed{xyz = C}$$

Choosing  $\frac{1}{x^2}, \frac{1}{y^2}, \frac{1}{z^2}$  as multipliers of each fraction of equation (1), we get

$$\frac{\frac{dx}{x^2}}{y-z} = \frac{\frac{dy}{y^2}}{z-x} = \frac{\frac{dz}{z^2}}{x-y} = \frac{\frac{dx}{x^2} + \frac{dy}{y^2} + \frac{dz}{z^2}}{\cancel{y-z} + \cancel{z-x} + \cancel{x-y}}$$

$$\Rightarrow \frac{dx}{x^2} + \frac{dy}{y^2} + \frac{dz}{z^2} = 0$$

$$\Rightarrow \frac{1}{x} + \frac{1}{y} + \frac{1}{z} = K$$

$$\text{Integration } \int \frac{dx}{x^2} + \int \frac{dy}{y^2} + \int \frac{dz}{z^2} = 0$$

$$\therefore \text{Soln: } \Phi(xyz, \frac{1}{x} + \frac{1}{y} + \frac{1}{z}) = 0$$